\documentclass{article}
\usepackage{chemfig}
\usepackage{amsmath}
\usepackage{amssymb}
\usepackage{xcolor}
\usepackage{chemfig}
\usepackage[version=4]{mhchem}
\begin{document}

\schemestart
    A 
    \arrow(A--B){<=>[*{90} $k_{AB}$][*{90} $k_{BA}$]}[-90,1.5] 
    B
    \arrow(@B--C){<=>[$k_{BC}$][$k_{CB}$]}[,1.5]
    C
    \arrow(@C--D){<=>[$k_{CD}$][$k_{DC}$]}[90,1.5]
    D
    \arrow(@A--@D){<=>[$k_{AD}$][$k_{DA}$]}[,1]
    \arrow(@A--@C){<=>[$k_{AC}$][$k_{CA}$]}[,1]
\schemestop

\section{asd}
$$
M_{ij} = k_{ji} - \delta_{ij}\sum_{k=1}^N k_{ik}
$$

$$
\frac{\prod_{\; \;}k_{ij}}{\prod_{\; \;}k_{ji}}
= \exp\left({\frac{\Delta \mu}{T}}\right)
$$

$$
X(t) \in \mathbb{N}
$$

$$
\frac{d}{dt} \langle X^k(t)\rangle
=\sum_{x,y\in\mathbb{N}}p_x(t)w_{xy}\left(y^k-x^k\right)
$$

$$
w_{xy} = w_{\Delta x=y-x} 
= \sum_{(i \rightarrow j) \in R_{\Delta x}}p_i(t)k_{ij}
$$

$$
\langle X(t)\rangle
= t \sum_{\Delta x, R_{\Delta x}} \Delta x p_i(t) k_{ij} \left(+ \langle X(0)\rangle\right)
$$

$$
\mathrm{Var}\left(X(t)\right)
= t \sum_{\Delta x, R_{\Delta x}} (\Delta x)^2 p_i(t) k_{ij} \left(+ \mathrm{Var}\left(X(0)\right)\right)
$$

$$
\tau \sim \mathrm{Exp}(k_i)
$$

$$
j^* \sim \mathrm{WeightedSampling}\left(\frac{k_{ij^*}}{k_i}\right)
$$

$$
k_i := \sum_j k_{ij}
$$

\begin{equation}
\begin{split} 
\frac{k_{DT}}{k_{TD}}
&= \left.\frac{k_{DT}}{k_{TD}}\right|_{eq.}
\left(
\frac{[T]}{[D]}
\middle/
\left.\frac{[T]}{[D]}\right|_{eq.}
\right)
\end{split}
\end{equation}
% 
%&=\frac{K_d^D}{K_d^T} \frac{[T]}{[D]}
%\left(
%\left.\frac{[T]}{[D]}\right|_{eq.}
%\middle/
%\left.\frac{[T]}{[D]}\right|_{eq.}
%\right)\\

$$
\Delta\mu \propto \log
\left(
\frac{[T]}{[D]}
\middle/
\left.\frac{[T]}{[D]}\right|_{eq.}
\right)
$$

\begin{equation}
\begin{split}
&r_{ATP}
    \propto \left(1 - \left.\frac{[T]}{[D]}\right|_{eq.}\bigg/\frac{[T]}{[D]}\right) k_h k_\uparrow k_{DT} \\
&\langle v \rangle = \Delta x \cdot r_{ATP}  
\end{split}
\end{equation}

\begin{equation}
\begin{split}
&\mathcal{L} = \frac{1}{2}k \sum_{i=1}^{N-1} (h_i - h_0)^2 + \frac{1}{2}k' (h_N - h_0)^2 - \lambda \sum_{i=1}^N h_i \\
&\implies
\begin{cases}
    h_{i\neq N} = h_0 \frac{k-k'}{(N-1)k'+k}, & \\
    h_N = -(N-1) h_{i\neq N} &
\end{cases}
\end{split}
\end{equation}

\vspace*{0.5cm}
\begin{center}
    \schemestart
    A
    \arrow(FlatT--FlatD){<->>[*0 $\textcolor{red}{\bar{k}_h}$][*0 $k_s$]}[-90,1.1] 
    B
    \arrow(@FlatD--ExtendedD){<->>[$k_{\uparrow ext.}$][$k_{\downarrow cont.}$]}[,1.1]
    C
    \arrow(@ExtendedD--ExtendedT){<->>[*0 $k_{DT}$][*0 $k_{TD}$]}[90,1.1]
    D
    \arrow(@FlatT--@ExtendedT){<<->[$\textcolor{red}{\bar{k}_{\downarrow ext.}}$][$k_{\uparrow cont.}$]}[,1.1]
\schemestop
\end{center}
\vspace*{0.5cm}

$$
\Delta h = 2 \implies \Delta x = 10
$$

\begin{equation}
\begin{split}
&r_{ATP}
    \propto \left(1 - \left.\frac{[T]}{[D]}\right|_{eq.}\bigg/\frac{[T]}{[D]}\right) \bar{k}_h k_{\uparrow ext.} k_{DT} k_{\uparrow cont.} \\
&\langle v \rangle = \Delta x \cdot r_{ATP}  
\end{split}
\end{equation}

\begin{equation}
\begin{split}
&r_{ATP}
    \propto \left(1 - \left.\frac{[T]}{[D]}\right|_{eq.}\bigg/\frac{[T]}{[D]}\right) \prod \; \; k \\
&\langle v \rangle = \Delta x \cdot r_{ATP}  
\end{split}
\end{equation}

\begin{center}
    \schemestart
        A
        \arrow(A--B){<->>[*0 $k_h$][*0 $k_s$]}[-90,1] 
        B
    \schemestop
    \chemmove{
        \draw[red,shorten <=8pt,shorten >=8pt]
        (A).. controls +(-45:10mm) and +(45:10mm).. 
        node[shift=(0:4mm)] {$k_{TD}$} (B);
    }
\end{center}

\begin{equation}
\begin{cases}
    p_A \propto k_s k_{DT} + k_\downarrow k_s + k_\uparrow k_{DT} \\
    p_B \propto k_h k_\downarrow + k_{DT} k_h + k_{TD} k_\downarrow \\
    p_C \propto k_\uparrow k_{TD} + k_s k_{TD} + k_h k_\uparrow
\end{cases}
\end{equation}

\begin{equation}
\begin{cases}
    p_A \propto k_s \\
    p_B \propto k_h + k_{TD}
\end{cases}
\end{equation}

$$
k, k'
$$

\begin{equation}
\left\{
\begin{split}
    \frac{d[\text{PT}]}{dt} &= k_{on}^T [\text{P}][\text{T}] - k_{off}^T [\text{PT}] \\
    \frac{d[\text{PD}]}{dt} &= k_{on}^D [\text{P}][\text{D}] - k_{off}^D [\text{PD}] \\
    \frac{d[\text{P}]}{dt} &= k_{off}^T [\text{PT}] + k_{off}^D [\text{PD}] - (k_{on}^T + k_{on}^D) [\text{P}]
\end{split}
\right.
\end{equation}

$\Delta x = 2$ a.a.

$\Delta x = 10$ a.a.


\end{document}